Assert macros

theories/examples/macros/assert.v
@@ -1,12 +1,12 @@
-From iris.algebra Require Import frac.
 From iris.proofmode Require Import proofmode.
-From cap_machine Require Import logrel addr_reg_sample fundamental rules proofmode.
+From cap_machine Require Import logrel rules proofmode.
+From cap_machine Require Import fetch.
 
 (* Assert routine *)
 
 (* Maintains a flag storing whether an assert has failed. *)
 
-Section Assert.
+Section Assert_subroutine.
   Context
     {Σ : gFunctors}
       {ceriseg: ceriseG Σ}
@@ -14,23 +14,25 @@ Section Assert.
       {MP: MachineParameters}
   .
 
-  (* assert (r4 == r5) *)
-  Definition assert_subroutine_instrs :=
+  (* Asserts (rsrc1 == rsrc2).
+     Jumps back to rret.
+   *)
+  Definition assert_subroutine_instrs (rret rsrc1 rsrc2 : RegName) :=
     encodeInstrsW [
-      Sub r_t4 r_t4 r_t5;
-      Jnz 4 r_t4;
+      Sub rsrc1 rsrc1 rsrc2;
+      Jnz 4 rsrc1;
       (* success case *)
-      Mov r_t4 0;
-      Mov r_t5 0;
-      Jalr cra r_t0; (* return *)
+      Mov rsrc1 0;
+      Mov rsrc2 0;
+      JmpCap rret; (* return *)
       (* failure case *)
-      Mov r_t5 PC; (* pointer to cap: *)
-      Lea r_t5 7; (* pointer to cap: *)
-      Load r_t5 r_t5;
-      Store r_t5 1;
-      Mov r_t4 0;
-      Mov r_t5 0;
-      Jalr cra r_t0 (* return *)
+      Mov rsrc2 PC; (* pointer to cap: *)
+      Lea rsrc2 7; (* pointer to cap: *)
+      Load rsrc2 rsrc2;
+      Store rsrc2 1;
+      Mov rsrc1 0;
+      Mov rsrc2 0;
+      JmpCap rret (* return *)
     ].
   (* followed in memory by:
     cap: (RW, flag, end, flag)
@@ -38,53 +40,58 @@ Section Assert.
     end:
   *)
 
-  Definition assert_inv (b a_flag e : Addr) : iProp Σ :=
+  Definition assert_inv (rret rsrc1 rsrc2 : RegName) (b_assert e_assert a_flag : Addr) : iProp Σ :=
     (∃ cap_addr,
-       codefrag b assert_subroutine_instrs ∗
-       ⌜(b + length assert_subroutine_instrs)%a = Some cap_addr⌝ ∗
+       codefrag b_assert (assert_subroutine_instrs rret rsrc1 rsrc2) ∗
+       ⌜(b_assert + length (assert_subroutine_instrs rret rsrc1 rsrc2))%a = Some cap_addr⌝ ∗
        ⌜(cap_addr + 1)%a = Some a_flag⌝ ∗
-       ⌜(a_flag + 1)%a = Some e⌝ ∗
-       cap_addr ↦ₐ WCap RW Global a_flag e a_flag).
+       ⌜(a_flag + 1)%a = Some e_assert⌝ ∗
+       cap_addr ↦ₐ WCap RW Global a_flag e_assert a_flag).
 
-  Lemma assert_subroutine_spec g b a_flag e cont n1 n2 flag N E φ :
+  Lemma assert_subroutine_spec
+    (rret rsrc1 rsrc2 : RegName)
+    (pc_g : Locality) (pc_b pc_e a_flag : Addr)
+    ( n1 n2 flag : Z ) ( wret : Word)
+    (N : namespace) (E : coPset) (φ : language.val cap_lang -> iProp Σ) :
     ↑N ⊆ E →
-    (  na_inv logrel_nais N (assert_inv b a_flag e)
+    (  na_inv logrel_nais N (assert_inv rret rsrc1 rsrc2 pc_b pc_e a_flag)
      ∗ na_own logrel_nais E
-     ∗ PC ↦ᵣ WCap RX g b e b
-     ∗ (∃ wcra, cra ↦ᵣ wcra)
-     ∗ r_t0 ↦ᵣ cont
-     ∗ r_t4 ↦ᵣ WInt n1
-     ∗ r_t5 ↦ᵣ WInt n2
+     ∗ PC ↦ᵣ WCap RX pc_g pc_b pc_e pc_b
+     ∗ rret ↦ᵣ wret
+     ∗ rsrc1 ↦ᵣ WInt n1
+     ∗ rsrc2 ↦ᵣ WInt n2
      ∗ a_flag ↦ₐ WInt flag
      ∗ ▷ (na_own logrel_nais E
-          ∗ PC ↦ᵣ updatePcPerm cont
-          ∗ (∃ wcra, cra ↦ᵣ wcra)
-          ∗ r_t0 ↦ᵣ cont
-          ∗ r_t4 ↦ᵣ WInt 0
-          ∗ r_t5 ↦ᵣ WInt 0
+          ∗ PC ↦ᵣ updatePcPerm wret
+          ∗ rret ↦ᵣ wret
+          ∗ rsrc1 ↦ᵣ WInt 0
+          ∗ rsrc2 ↦ᵣ WInt 0
           ∗ a_flag ↦ₐ WInt (if (n1 =? n2)%Z then flag else 1%Z)
           -∗ WP Seq (Instr Executable) {{ φ }})
      ⊢ WP Seq (Instr Executable) {{ φ }})%I.
   Proof.
-    iIntros (HNE) "(#Hinv & Hna & HPC & Hcra & Hr0 & Hr1 & Hr2 & Hflag & Hφ)".
-    iDestruct "Hcra" as (wcra) "Hcra".
+    iIntros (HNE) "(#Hinv & Hna & HPC & Hrdst & Hrsrc1 & Hrsrc2 & Hflag & Hφ)".
     iMod (na_inv_acc with "Hinv Hna") as "(>Hassert & Hna & Hinv_close)"; auto.
     iDestruct "Hassert" as (cap_addr) "(Hprog & %Hcap & %Hflag & %He & Hcap)".
-    rewrite /assert_subroutine_instrs. codefrag_facts "Hprog".
-    assert (SubBounds b e b (b ^+ length assert_subroutine_instrs)%a) by solve_addr.
+    rewrite /assert_subroutine_instrs.
+    codefrag_facts "Hprog". rename H into HcontProg.
+    assert (SubBounds pc_b pc_e
+              pc_b (pc_b ^+ length (assert_subroutine_instrs rret rsrc1 rsrc2))%a)
+      as HsubBounds by solve_addr.
     iInstr "Hprog".
-    destruct (decide (n1 = n2)).
+    destruct (decide (n1 = n2)) as [Heq|Heq].
     { (* n1 = n2 *)
       subst n2. rewrite (_: n1 - n1 = 0)%Z; last lia.
       iGo "Hprog".
       iMod ("Hinv_close" with "[Hprog Hcap $Hna]") as "Hna".
       { iExists _. iNext. iFrame. iPureIntro. repeat split; solve_addr. }
+
       iApply "Hφ". iFrame. rewrite Z.eqb_refl //. }
     { (* n1 ≠ n2 *)
       iInstr "Hprog". { assert (n1 - n2 ≠ 0)%Z by lia. congruence. }
       iInstr "Hprog".
       iInstr "Hprog".
-      rewrite (_: (b ^+ 12)%a = cap_addr); [|solve_addr].
+      rewrite (_: (pc_b ^+ 12)%a = cap_addr); [|solve_addr].
       iInstr "Hprog"; first solve_addr.
       iInstr "Hprog"; first solve_addr.
       iGo "Hprog".
@@ -94,37 +101,131 @@ Section Assert.
       by apply Z.eqb_neq. }
   Qed.
 
-  Lemma assert_success_spec g b a_flag e cont n1 n2 N E φ :
+  Lemma assert_subroutine_success_spec
+    (rret rsrc1 rsrc2 : RegName)
+    (pc_g : Locality) (pc_b pc_e a_flag : Addr)
+    ( n1 n2 flag : Z ) ( wret : Word)
+    (N : namespace) (E : coPset) (φ : language.val cap_lang -> iProp Σ) :
     ↑N ⊆ E →
     n1 = n2 →
-    (  na_inv logrel_nais N (assert_inv b a_flag e)
+    (  na_inv logrel_nais N (assert_inv rret rsrc1 rsrc2 pc_b pc_e a_flag)
      ∗ na_own logrel_nais E
-     ∗ PC ↦ᵣ WCap RX g b e b
-     ∗ (∃ wcra, cra ↦ᵣ wcra)
-     ∗ r_t0 ↦ᵣ cont
-     ∗ r_t4 ↦ᵣ WInt n1
-     ∗ r_t5 ↦ᵣ WInt n2
+     ∗ PC ↦ᵣ WCap RX pc_g pc_b pc_e pc_b
+     ∗ rret ↦ᵣ wret
+     ∗ rsrc1 ↦ᵣ WInt n1
+     ∗ rsrc2 ↦ᵣ WInt n2
      ∗ ▷ (na_own logrel_nais E
-          ∗ PC ↦ᵣ updatePcPerm cont
-          ∗ (∃ wcra, cra ↦ᵣ wcra)
-          ∗ r_t0 ↦ᵣ cont
-          ∗ r_t4 ↦ᵣ WInt 0
-          ∗ r_t5 ↦ᵣ WInt 0
+          ∗ PC ↦ᵣ updatePcPerm wret
+          ∗ rret ↦ᵣ wret
+          ∗ rsrc1 ↦ᵣ WInt 0%Z
+          ∗ rsrc2 ↦ᵣ WInt 0%Z
           -∗ WP Seq (Instr Executable) {{ φ }})
      ⊢ WP Seq (Instr Executable) {{ φ }})%I.
   Proof.
-    iIntros (HNE Heq) "(#Hinv & Hna & HPC & Hcra & Hr0 & Hr1 & Hr2 & Hφ)".
-    iDestruct "Hcra" as (wcra) "Hcra".
+    iIntros (HNE Heq) "(#Hinv & Hna & HPC & Hrdst & Hrsrc1 & Hrsrc2 & Hφ)".
     iMod (na_inv_acc with "Hinv Hna") as "(>Hassert & Hna & Hinv_close)"; auto.
     iDestruct "Hassert" as (cap_addr) "(Hprog & %Hcap & %Hflag & %He & Hcap)".
     rewrite /assert_subroutine_instrs. codefrag_facts "Hprog".
-    assert (SubBounds b e b (b ^+ length assert_subroutine_instrs)%a) by solve_addr.
+    assert (SubBounds pc_b pc_e
+              pc_b (pc_b ^+ length (assert_subroutine_instrs rret rsrc1 rsrc2))%a)
+      as HsubBounds by solve_addr.
     iInstr "Hprog".
     rewrite (_: n1 - n2 = 0)%Z; last lia.
     iGo "Hprog".
     iMod ("Hinv_close" with "[Hprog Hcap $Hna]") as "Hna".
     { iExists _. iNext. iFrame. iPureIntro. repeat split; solve_addr. }
     iApply "Hφ". iFrame.
+  Qed.
+
+End Assert_subroutine.
+
+Section Assert.
+  Context
+    {Σ : gFunctors}
+      {ceriseg: ceriseG Σ}
+      {nainv: logrel_na_invs Σ}
+      {MP: MachineParameters}
+  .
+
+  (* assert macros:
+   - fetch the assert entry point an the n-th position in the import table
+   - execute the assert subroutine
+
+   - rret, rsrc1 and rsrc2 are all clobbered
+   *)
+  Definition assert_instrs (n : Z) (rdst rscratch1 rscratch2 rsrc1 rsrc2 : RegName) :=
+    fetch_instrs n rdst rscratch1 rscratch2 ++
+    encodeInstrsW [
+      Jalr rscratch1 rdst;
+      Mov rscratch1 0%Z;
+      Mov rdst 0%Z
+    ].
+
+  Lemma updatePcPerm_seal_perm_sentry (p : Perm) (g : Locality) (b e a : Addr) :
+    isSentry p = false ->
+    updatePcPerm (WCap (seal_perm_sentry p) g b e a) = WCap p g b e a.
+  Proof.
+    intros Hsentry.
+    destruct p; auto.
+    by cbn in Hsentry.
+  Qed.
+
+  Lemma assert_success_spec
+    (n : Z) (rdst rscratch1 rscratch2 rsrc1 rsrc2 : RegName)
+    (pc_g : Locality) (pc_p : Perm) (pc_b pc_e pc_a : Addr)
+    (g_assert : Locality) (b_assert e_assert a_flag : Addr)
+    (n1 n2 flag : Z) (wdst w1 w2 : Word)
+    (N : namespace) (E : coPset) (φ : language.val cap_lang -> iProp Σ) :
+
+    let assert_macro := assert_instrs n rdst rscratch1 rscratch2 rsrc1 rsrc2 in
+    let a_last := (pc_a ^+ length assert_macro)%a in
+    executeAllowed pc_p = true →
+    SubBounds pc_b pc_e pc_a a_last →
+    withinBounds pc_b pc_e (pc_b ^+ n)%a = true ->
+
+    ↑N ⊆ E →
+    n1 = n2 →
+    (  na_inv logrel_nais N (assert_inv rscratch1 rsrc1 rsrc2 b_assert e_assert a_flag)
+     ∗ na_own logrel_nais E
+     ∗ PC ↦ᵣ WCap pc_p pc_g pc_b pc_e pc_a
+     ∗ rdst ↦ᵣ wdst
+     ∗ rscratch1 ↦ᵣ w1
+     ∗ rscratch2 ↦ᵣ w1
+     ∗ rsrc1 ↦ᵣ WInt n1
+     ∗ rsrc2 ↦ᵣ WInt n2
+     ∗ codefrag pc_a assert_macro
+     ∗ (pc_b ^+ n)%a ↦ₐ (WCap E_RX g_assert b_assert e_assert b_assert)
+     ∗ ▷ (na_own logrel_nais E
+          ∗ PC ↦ᵣ WCap pc_p pc_g pc_b pc_e a_last
+          ∗ rdst ↦ᵣ WInt 0
+          ∗ rscratch1 ↦ᵣ WInt 0
+          ∗ rscratch2 ↦ᵣ WInt 0
+          ∗ rsrc1 ↦ᵣ WInt 0
+          ∗ rsrc2 ↦ᵣ WInt 0
+          ∗ codefrag pc_a assert_macro
+          -∗ WP Seq (Instr Executable) {{ φ }})
+     ⊢ WP Seq (Instr Executable) {{ φ }})%I.
+  Proof.
+    intros assert_macro a_last; subst assert_macro a_last.
+    iIntros (Hpc_exec HsubBounds Hinbounds HNE Heq)
+      "(#Hinv & Hna & HPC & Hrdst & Hrscratch1 & Hrscratch2 & Hrsrc1 & Hrsrc2 & Hcode & Hpc_bn & Hφ)".
+    codefrag_facts "Hcode".
+    rewrite /assert_instrs.
+    focus_block_0 "Hcode" as "Hfetch" "Hcont".
+    iApply (fetch_spec with "[-]"); eauto; iFrame.
+    iNext; iIntros "(HPC & Hrdst & Hrscratch1 & Hrscratch2 & Hfetch & Hpc_bn)".
+    unfocus_block "Hfetch" "Hcont" as "Hcode".
+    focus_block 1 "Hcode" as a_assert Ha_assert "Hassert" "Hcont".
+    iGo "Hassert".
+    rewrite load_word_sentry.
+    iEval (cbn) in "HPC".
+    iApply (assert_subroutine_success_spec with "[-]"); eauto; iFrame "#∗".
+    iNext; iIntros "(Hna & HPC & Hrscratch1 & Hrsrc1 & Hrsrc2)".
+    rewrite updatePcPerm_seal_perm_sentry; last solve_pure.
+    iGo "Hassert".
+    unfocus_block "Hassert" "Hcont" as "Hcode".
+    replace (a_assert ^+ 3)%a with (pc_a ^+ 12)%a by solve_addr.
+    iApply "Hφ"; iFrame.
   Qed.
 
 End Assert.
